src/n_bit/numeral_bitsScript.sml
@@ -14,20 +14,10 @@ val SUC_RULE = CONV_RULE numLib.SUC_TO_NUMERAL_DEFN_CONV;
 
 (* -------------------------------------------------------- *)
 
-val iMOD_2EXP_def =
- Prim_rec.new_recursive_definition
-  {name = "iMOD_2EXP_def",
-   def = ``(iMOD_2EXP 0 n = 0) /\
-           (iMOD_2EXP (SUC x) n =
-              2 * (iMOD_2EXP x (n DIV 2)) + SBIT (ODD n) 0)``,
-   rec_axiom = prim_recTheory.num_Axiom};
+val SIMP_BIT1 = (GSYM o SIMP_RULE arith_ss []) BIT1;
 
 val iBITWISE_def =
   Definition.new_definition("iBITWISE_def", ``iBITWISE = BITWISE``);
-
-(* -------------------------------------------------------- *)
-
-val SIMP_BIT1 = (GSYM o SIMP_RULE arith_ss []) BIT1;
 
 val iBITWISE = prove(
   `(!opr a b. iBITWISE 0 opr a b = ZERO) /\
@@ -66,76 +56,6 @@ val DIV_2EXP = prove(
 );
 
 val NUMERAL_DIV_2EXP = save_thm("NUMERAL_DIV_2EXP", SUC_RULE DIV_2EXP);
-
-(* -------------------------------------------------------- *)
-
-val ADD_DIV_ADD_DIV2 = (GEN_ALL o ONCE_REWRITE_RULE [MULT_COMM] o
-                        SIMP_RULE arith_ss [GSYM ADD1] o SPECL [`n`,`1`] o
-                        SIMP_RULE bool_ss [DECIDE (Term `0 < 2`)] o SPEC `2`) ADD_DIV_ADD_DIV;
-
-val SPEC_MOD_COMMON_FACTOR = (GEN_ALL o SIMP_RULE arith_ss [GSYM EXP,ZERO_LT_TWOEXP] o
-            SPECL [`2`,`m`,`2 ** SUC h`]) MOD_COMMON_FACTOR;
-val SPEC_MOD_COMMON_FACTOR2 = (GEN_ALL o SYM o SIMP_RULE arith_ss [GSYM EXP,ZERO_LT_TWOEXP] o
-            SPECL [`2`,`m`,`2 ** h`]) MOD_COMMON_FACTOR;
-
-val SPEC_MOD_PLUS = (GEN_ALL o GSYM o SIMP_RULE bool_ss [ZERO_LT_TWOEXP] o SPEC `2 EXP n`) MOD_PLUS;
-val SPEC_TWOEXP_MONO = prove(
-  `!b. 1 < 2 ** SUC b`,
-  METIS_TAC [TWOEXP_MONO, EXP, prim_recTheory.LESS_0])
-
-val lem = prove(
-  `!m n. (2 * m) MOD 2 ** SUC n + 1 < 2 ** SUC n`,
-  RW_TAC arith_ss [SPEC_MOD_COMMON_FACTOR2,EXP,DOUBLE_LT,MOD_2EXP_LT,
-                   (GEN_ALL o numLib.REDUCE_RULE o SPECL [`m`,`i`,`1`]) LESS_MULT_MONO]
-);
-
-val BITS_SUC2 = prove(
-  `!h n. BITS (SUC h) 0 n = 2 * BITS h 0 (n DIV 2) + SBIT (ODD n) 0`,
-  RW_TAC arith_ss [SBIT_def]
-    THEN FULL_SIMP_TAC arith_ss [GSYM EVEN_ODD,EVEN_EXISTS,ODD_EXISTS,BITS_ZERO3,ADD_DIV_ADD_DIV2,
-                                 ONCE_REWRITE_RULE [MULT_COMM] MULT_DIV,SPEC_MOD_COMMON_FACTOR]
-    THEN SUBST1_TAC (SPEC `2 * m` ADD1)
-    THEN ONCE_REWRITE_TAC [SPEC_MOD_PLUS]
-    THEN SIMP_TAC bool_ss [LESS_MOD,ZERO_LT_TWOEXP,SPEC_TWOEXP_MONO,LESS_MOD,lem]
-);
-
-val MOD_2EXP_ZERO = prove(
-  `!x. MOD_2EXP x 0 = 0`,
-  SIMP_TAC arith_ss [MOD_2EXP_def,ZERO_MOD,ZERO_LT_TWOEXP]
-);
-
-val iMOD_2EXP = prove(
-  `!x n. MOD_2EXP x (NUMERAL n) = NUMERAL (iMOD_2EXP x n)`,
-  REWRITE_TAC [NUMERAL_DEF]
-    THEN Induct
-    THEN1 SIMP_TAC arith_ss [iMOD_2EXP_def,MOD_2EXP_def]
-    THEN STRIP_TAC THEN REWRITE_TAC [iMOD_2EXP_def]
-    THEN POP_ASSUM (SUBST1_TAC o SYM o SPEC `n DIV 2`)
-    THEN Cases_on `x`
-    THEN1 (SIMP_TAC arith_ss [MOD_2EXP_def,MOD_2,EVEN_ODD,SBIT_def] THEN PROVE_TAC [])
-    THEN REWRITE_TAC [(GSYM o REWRITE_RULE [GSYM MOD_2EXP_def]) BITS_ZERO3,BITS_SUC2]
-);
-
-val iMOD_2EXP_CLAUSES = prove(
-  `(!n. iMOD_2EXP 0 n = ZERO) /\
-   (!x n. iMOD_2EXP x ZERO = ZERO) /\
-   (!x n. iMOD_2EXP (SUC x) (BIT1 n) = BIT1 (iMOD_2EXP x n)) /\
-   (!x n. iMOD_2EXP (SUC x) (BIT2 n) = iDUB (iMOD_2EXP x (SUC n)))`,
-  RW_TAC arith_ss [iMOD_2EXP_def,iDUB,SBIT_def,numeral_evenodd,GSYM DIV2_def,
-                   REWRITE_RULE [SYM ALT_ZERO,NUMERAL_DEF,ADD1] NUMERAL_DIV2]
-    THENL [
-      REWRITE_TAC [ALT_ZERO],
-      REWRITE_TAC [ALT_ZERO]
-        THEN REWRITE_TAC [MOD_2EXP_ZERO,(GSYM o REWRITE_RULE [NUMERAL_DEF]) iMOD_2EXP],
-      SIMP_TAC arith_ss [SPEC `iMOD_2EXP x n` BIT1],
-      ONCE_REWRITE_TAC [(SYM o REWRITE_CONV [NUMERAL_DEF]) ``1``]
-        THEN REWRITE_TAC [ADD1]
-    ]
-);
-
-val iMOD_2EXP = save_thm("iMOD_2EXP",CONJ MOD_2EXP_ZERO iMOD_2EXP);
-
-val NUMERAL_MOD_2EXP = save_thm("NUMERAL_MOD_2EXP", SUC_RULE iMOD_2EXP_CLAUSES);
 
 (* -------------------------------------------------------- *)
 
@@ -198,8 +118,7 @@ val _ =
      ::
      map (DEFN o PURE_REWRITE_RULE [arithmeticTheory.NUMERAL_DEF,
                                GSYM arithmeticTheory.ALT_ZERO])
-         [NUMERAL_DIV2,iBITWISE, NUMERAL_BITWISE,
-          NUMERAL_MOD_2EXP,iMOD_2EXP, NUMERAL_DIV_2EXP])
+         [NUMERAL_DIV2,iBITWISE, NUMERAL_BITWISE, NUMERAL_DIV_2EXP])
  end;
 
 val _ = export_theory();
